$x=\ln y$
$y=e^{x}=g^{-1}(x)$
$F_{x}(x)=P(X \leq x)=P(\ln Y \leq x)$
$=P\left(y \leq e^{x}\right)$
$=\int_{-\infty}^{e^{x}} e^{-y} d y$
$=\int_{0}^{e^{x}} e^{-y} d y=F_{y}\left(e^{x}\right)$
$=\left[-e^{-y}\right]_{0}^{e^{x}}$
$=-e^{-e^{x}}+1$
$f_{x}(x)=\left\{\begin{array}{cc}e^{x} \cdot e^{-e^{x}}, & , x \in \mathbb{R}^{-x} \\ 0 & , \text { other wise }\end{array}\right.$
$\frac{d}{d x}\left(-e^{-e^{x}}\right)=\frac{d}{d}\left(-e^{x}\right) \cdot-e^{-e^{x}}$
$=-e^{x},-e^{-e^{x}}$
$=e^{x} \cdot e^{-e^{x}}$