\pdfminorversion=4
\documentclass[]{article}
\usepackage[utf8]{inputenc}
\usepackage{amssymb,latexsym,amsmath}
\usepackage[a4paper,top=3cm,bottom=2cm,left=3cm,right=3cm,marginparwidth=1.75cm]{geometry}
\usepackage{graphicx}
\usepackage[colorlinks=true, allcolors=blue]{hyperref}
\begin{document}

Given that $X=\ln Y$, it is strictly monotone, it is increasing on $(0, \infty)$ Thus we can directly apply Monotone Transformation Theorem \\
\\
$f_x(x)=\left\{\begin{array}{lll}f_y\left(g^{-1}(x)\right) \cdot\left|\frac{d}{d x} g^{-1}(x)\right| & \text { if } y=g(x) & x=\ln y=g(y) \\ 0 & \text { if } y \neq g(x) & y=e^x=g^{-1}(x)\end{array}\right.$\\
$=\left\{\begin{array}{ll}e^{-e^x} \cdot\left|e^x\right|=e^{-e^x} \cdot e^x & \left(e^x>0\right) \\ 0& \text{omitted, because }y>0 \text{ and the pdf of x is always not zero.}\end{array}\right.

\end{document}