\pdfminorversion=4
\documentclass[]{article}
\usepackage[utf8]{inputenc}
\usepackage{amssymb,latexsym,amsmath}
\usepackage[a4paper,top=3cm,bottom=2cm,left=3cm,right=3cm,marginparwidth=1.75cm]{geometry}
\usepackage{graphicx}
\usepackage[colorlinks=true, allcolors=blue]{hyperref}
\begin{document}

\begin{math}
\begin{aligned}
&x=\ln Y\\
&F X(x)=P(x \leqslant x)=P(\ln Y \leqslant x)\\
&=P\left(0<Y \leqslant e^x\right)\\
&=\int_0^{e^x} e^{-y} d y\\
&=\quad\left[-e^{-y}\right]_0^{e^x}\\
&=-e^{-e^x}-\left(-e^{-0}\right)\\
&=-e^{-e^x}-(-1)\\
&F_x(x)=\left\{\begin{array}{c}
0, x-1-e^{-e^x} \\
1-e^x, e^x, x>0
\end{array}\right.\\
&\begin{aligned}
& \frac{d}{d x}\left(1-e^{-e^x}\right) \\
=& \frac{d}{d x}(1)-\frac{d}{d x}\left(e^{-e^x}\right)
\end{aligned} \quad f_x(x)=\left\{\begin{array}{cc}
e^x \cdot e^{-e^x}, & x \in \mathbb{R} \\
0, & \text { otherwbe }
\end{array}\right.\\
&=\frac{d}{d x}\left(-e^x\right)^x \cdot-e^{-e^x}
\end{aligned}
\end{math}

\end{document}