Given that $X=\ln Y$, it is strictly monotone, it is increasing on $(0, \infty)$ Thus we can directly apply Monotone Transformation Theorem
$f_{x}(x)=\left\{\begin{array}{lll}f_{y}\left(g^{-1}(x)\right) \cdot\left|\frac{d}{d x} g^{-1}(x)\right| & \text { if } y=g(x) & x=\ln y=g(y) \\ 0 \text { ify } y \neq g(x) & y=e^{x}=g^{-1}(x)\end{array}\right.$
$=\left\{\begin{array}{ll}e^{-e^{x}} \cdot\left|e^{x}\right|=e^{-e^{x}} \cdot e^{x} & \left(e^{x}>0\right) \\ 0 & \text { omitted, because } y>0\end{array} \quad\right.$ and the pdf of $x$ is always not zero.